utils/Zeta.BinTreePtr.fsti
@@ -6,7 +6,7 @@ open Zeta.BinTree
  * ptrfn is a function that maps each node and a direction (left | right) to an 
  * optional descendant in the corresponing (left|right) subtree
  *)
-type ptrfn = (n:bin_tree_node) -> (c:bin_tree_dir) -> option (d:bin_tree_node{is_desc d (child c n)})
+let ptrfn = n:bin_tree_node -> c:bin_tree_dir -> o:(option bin_tree_node){None = o \/ is_desc (Some?.v o) (child c n)}
 
 (* does n point to some node along direction c *)
 let points_to_some (pf:ptrfn) (n:bin_tree_node) (c:bin_tree_dir): bool = 
@@ -17,10 +17,11 @@ let pointed_node (pf:ptrfn) (n:bin_tree_node) (c:bin_tree_dir {points_to_some pf
   Some?.v (pf n c)
 
 (* does a point to d *)
-let points_to (pf: ptrfn) (d: bin_tree_node) (a: bin_tree_node{is_proper_desc d a}): bool = 
-  let c = desc_dir d a in
-  points_to_some pf a c && 
-  d = pointed_node pf a c 
+let points_to (pf: ptrfn) (d: bin_tree_node) (a: bin_tree_node): bool
+  = is_proper_desc d a && (
+        let c = desc_dir d a in
+        points_to_some pf a c &&
+        d = pointed_node pf a c)
 
 let points_to_none (pf:ptrfn) (n:bin_tree_node): bool = 
   not (points_to_some pf n Left) && 
@@ -49,6 +50,7 @@ val lemma_points_to_reachable (pf: ptrfn)
                               (a: bin_tree_node):
   Lemma (requires (is_proper_desc d a /\ points_to pf d a))
         (ensures (reachable pf d a))
+        [SMTPat (points_to pf d a)]
 
 (* pdesc is a transitive relation *)
 val lemma_reachable_transitive (pf: ptrfn) (a b c: bin_tree_node):
@@ -69,39 +71,96 @@ val lemma_non_reachable_desc_of_none (pf: ptrfn)
                                                       None? (pf a (desc_dir d a))}):
   Lemma (not (reachable pf d a))
 
+val lemma_desc_of_prev_not_reachable (pf:ptrfn)
+                                     (d1:bin_tree_node)
+                                     (a:bin_tree_node)
+                                     (d2:bin_tree_node):
+  Lemma (requires (reachable pf d1 a /\ d1 <> a /\
+                   is_proper_desc d1 d2 /\
+                   is_proper_desc d2 (prev_in_path pf d1 a)))
+        (ensures (not (reachable pf d2 a)))
+
+val lemma_points_to_not_reachable_between (pf:ptrfn)
+                                          (d:bin_tree_node)
+                                          (a:bin_tree_node)
+                                          (pd:bin_tree_node)
+                                          (n:bin_tree_node)
+  : Lemma (requires (reachable pf pd a /\
+                     is_proper_desc d pd /\
+                     points_to pf d pd /\
+                     is_proper_desc d n /\
+                     is_proper_desc n pd))
+          (ensures (not (reachable pf n a)))
+
+val lemma_points_to_is_prev (pf:ptrfn)
+                            (d:bin_tree_node)
+                            (a:bin_tree_node)
+                            (pd:bin_tree_node):
+  Lemma (requires (reachable pf d a /\
+                   reachable pf pd a /\
+                   is_proper_desc d pd /\
+                   d <> a /\
+                   points_to pf d pd))
+        (ensures (prev_in_path pf d a = pd))
+
+(*
+ * The setup is (Root -> a) and (Root -> d) and d is a proper descendant of a,
+ * then a points to some ancestor of d
+ *)
+val lemma_reachable_between (pf: ptrfn) (d: bin_tree_node) (a: bin_tree_node):
+  Lemma (requires (root_reachable pf d /\ is_proper_desc d a /\ root_reachable pf a))
+        (ensures (let c = desc_dir d a in
+                  points_to_some pf a c /\
+                  is_desc d (pointed_node pf a c)))
+
+(* a rooted pointer function is where the set of edges form a tree from the root *)
+let rooted (pf:ptrfn)
+  = forall (d a: bin_tree_node). {:pattern points_to pf d a} points_to pf d a ==> root_reachable pf a
+
+val rooted_implies_root_reachable_dest (pf:ptrfn {rooted pf}) (d a: _)
+  : Lemma (ensures (points_to pf d a ==> root_reachable pf d))
+          [SMTPat (points_to pf d a)]
+
 (* Extend the pointer function with a new points_to edge *)
 let extend_ptrfn 
   (pf:ptrfn) 
   (d:bin_tree_node{points_to_none pf d}) 
   (a:bin_tree_node{is_proper_desc d a /\
-                   not (points_to_some pf a (desc_dir d a)) /\
-                   root_reachable pf a}): ptrfn = 
-  let c = desc_dir d a in
-  fun n' c' -> if n' = a && c' = c then Some d else pf n' c'
+                   not (points_to_some pf a (desc_dir d a))})
+  : ptrfn
+  = let c = desc_dir d a in
+    fun n' c' -> if n' = a && c' = c then Some d else pf n' c'
+
+(* characterize points to in extend_ptrfn *)
+val extend_ptrfn_edges
+  (pf:ptrfn)
+  (d:bin_tree_node{points_to_none pf d})
+  (a:bin_tree_node{is_proper_desc d a /\
+                   not (points_to_some pf a (desc_dir d a))})
+  (d' a': bin_tree_node)
+  : Lemma (ensures (let pfe = extend_ptrfn pf d a in
+                    (points_to pf d' a' ==> points_to pfe d' a') /\
+                    (points_to pfe d' a' ==> ~ (points_to pf d' a') ==> d' = d /\ a' = a)))
 
 (* extension does not reduce reachability *)
 val lemma_extend_reachable 
   (pf:ptrfn) 
   (d:bin_tree_node{points_to_none pf d}) 
   (a:bin_tree_node{is_proper_desc d a /\ 
-                   not (points_to_some pf a (desc_dir d a)) /\
-                   root_reachable pf a})
+                   not (points_to_some pf a (desc_dir d a))})
   (n: bin_tree_node):
-  Lemma (requires (root_reachable pf n))
-        (ensures (root_reachable (extend_ptrfn pf d a) n))
+  Lemma (ensures (root_reachable pf n ==> root_reachable (extend_ptrfn pf d a) n))
 
-(* extension adds reachability to the new node *)
-val lemma_extend_reachable_new
-  (pf:ptrfn) 
-  (d:bin_tree_node{points_to_none pf d}) 
-  (a:bin_tree_node{is_proper_desc d a /\ 
-                   not (points_to_some pf a (desc_dir d a)) /\
-                   root_reachable pf a}):
-  Lemma (root_reachable (extend_ptrfn pf d a) d)
-  
+val lemma_extend_rooted
+  (pf:ptrfn{rooted pf})
+  (d:bin_tree_node{points_to_none pf d})
+  (a:bin_tree_node{is_proper_desc d a /\
+                   not (points_to_some pf a (desc_dir d a))})
+  : Lemma (ensures (root_reachable pf a ==> rooted (extend_ptrfn pf d a)))
+
 (* extends confers reachability only to the new node *)
 val lemma_extend_not_reachable
-  (pf:ptrfn) 
+  (pf:ptrfn {rooted pf})
   (d:bin_tree_node{points_to_none pf d}) 
   (a:bin_tree_node{is_proper_desc d a /\ 
                    not (points_to_some pf a (desc_dir d a)) /\
@@ -116,8 +175,7 @@ let extendcut_ptrfn
   (d:bin_tree_node{points_to_none pf d})
   (a:bin_tree_node{is_proper_desc d a /\ 
                    points_to_some pf a (desc_dir d a) /\
-                   is_proper_desc (pointed_node pf a (desc_dir d a)) d /\
-                   root_reachable pf a}): ptrfn = 
+                   is_proper_desc (pointed_node pf a (desc_dir d a)) d}): ptrfn =
    let c1 = desc_dir d a in
    let d' = pointed_node pf a c1 in
    let c2 = desc_dir d' d in
@@ -131,11 +189,18 @@ val lemma_extendcut_reachable
   (d:bin_tree_node{points_to_none pf d})
   (a:bin_tree_node{is_proper_desc d a /\ 
                     points_to_some pf a (desc_dir d a) /\
-                    is_proper_desc (pointed_node pf a (desc_dir d a)) d /\ 
-                    root_reachable pf a})
+                    is_proper_desc (pointed_node pf a (desc_dir d a)) d})
   (n: bin_tree_node):
   Lemma (requires (root_reachable pf n))
         (ensures (root_reachable (extendcut_ptrfn pf d a) n))
+
+val lemma_extendcut_rooted
+  (pf:_{rooted pf})
+  (d:bin_tree_node{points_to_none pf d})
+  (a:bin_tree_node{is_proper_desc d a /\
+                    points_to_some pf a (desc_dir d a) /\
+                    is_proper_desc (pointed_node pf a (desc_dir d a)) d})
+  : Lemma (ensures (rooted (extendcut_ptrfn pf d a)))
 
 (* Root reachability is preserved with extendcut *)
 val lemma_extendcut_reachable_new
@@ -143,17 +208,15 @@ val lemma_extendcut_reachable_new
   (d:bin_tree_node{points_to_none pf d})
   (a:bin_tree_node{is_proper_desc d a /\ 
                     points_to_some pf a (desc_dir d a) /\
-                    is_proper_desc (pointed_node pf a (desc_dir d a)) d /\ 
-                    root_reachable pf a}):
-  Lemma (root_reachable (extendcut_ptrfn pf d a) d)
+                    is_proper_desc (pointed_node pf a (desc_dir d a)) d})
+  : Lemma (root_reachable pf a ==> root_reachable (extendcut_ptrfn pf d a) d)
 
 val lemma_extendcut_not_reachable 
-  (pf:ptrfn)
+  (pf:ptrfn {rooted pf})
   (d:bin_tree_node{points_to_none pf d})
   (a:bin_tree_node{is_proper_desc d a /\ 
                     points_to_some pf a (desc_dir d a) /\
-                    is_proper_desc (pointed_node pf a (desc_dir d a)) d /\ 
-                    root_reachable pf a})
+                    is_proper_desc (pointed_node pf a (desc_dir d a)) d})
   (n: bin_tree_node):
   Lemma (requires (not (root_reachable pf n) /\ n <> d))
         (ensures (not (root_reachable (extendcut_ptrfn pf d a) n)))
@@ -162,58 +225,15 @@ val lemma_extendcut_not_reachable
 let feq_ptrfn (pf1: ptrfn) (pf2: ptrfn) = 
   forall n. forall c. {:pattern (pf1 n c) \/ (pf2 n c)} pf1 n c == pf2 n c
 
-(* Two equal pointer functions have the same reachability relationship *)
-val lemma_reachable_feq (pf1: ptrfn) (pf2: ptrfn) (d: bin_tree_node) (a: bin_tree_node):
-  Lemma (requires (feq_ptrfn pf1 pf2))
-        (ensures (reachable pf1 d a = reachable pf2 d a))
-        [SMTPat (reachable pf1 d a); SMTPat (reachable pf2 d a)]
-
-val lemma_desc_of_prev_not_reachable (pf:ptrfn)
-                                     (d1:bin_tree_node)
-                                     (a:bin_tree_node)
-                                     (d2:bin_tree_node):
-  Lemma (requires (reachable pf d1 a /\ d1 <> a /\
-                   is_proper_desc d1 d2 /\
-                   is_proper_desc d2 (prev_in_path pf d1 a)))
-        (ensures (not (reachable pf d2 a)))
-
-val lemma_prev_in_path_feq (pf1: ptrfn) 
-                           (pf2: ptrfn) 
-                           (d:bin_tree_node) 
-                           (a:bin_tree_node):
-   Lemma (requires (feq_ptrfn pf1 pf2 /\ reachable pf1 d a /\ d <> a))
-         (ensures (prev_in_path pf1 d a = prev_in_path pf2 d a))
-
-val lemma_points_to_not_reachable_between (pf:ptrfn)
-                                          (d:bin_tree_node)
-                                          (a:bin_tree_node)
-                                          (pd:bin_tree_node)
-                                          (n:bin_tree_node)
-  : Lemma (requires (reachable pf pd a /\
-                     is_proper_desc d pd /\
-                     points_to pf d pd /\
-                     is_proper_desc d n /\
-                     is_proper_desc n pd))
-          (ensures (not (reachable pf n a)))
-                     
-val lemma_points_to_is_prev (pf:ptrfn)
-                            (d:bin_tree_node)
-                            (a:bin_tree_node)
-                            (pd:bin_tree_node):
-  Lemma (requires (reachable pf d a /\ 
-                   reachable pf pd a /\ 
-                   is_proper_desc d pd /\
-                   d <> a /\
-                   points_to pf d pd))
-        (ensures (prev_in_path pf d a = pd))
-
+val lemma_feq_implies_equal (pf1 pf2:_)
+  : Lemma (ensures (feq_ptrfn pf1 pf2 ==> pf1 == pf2))
+          [SMTPat (feq_ptrfn pf1 pf2)]
 
 val lemma_extend_prev
   (pf:ptrfn)
   (d:bin_tree_node{points_to_none pf d}) 
   (a:bin_tree_node{is_proper_desc d a /\ 
-                   not (points_to_some pf a (desc_dir d a)) /\
-                   root_reachable pf a})
+                   not (points_to_some pf a (desc_dir d a))})
   (n: bin_tree_node):
   Lemma (requires (root_reachable pf n /\ n <> d /\ n <> Root))
         (ensures (root_reachable (extend_ptrfn pf d a) n /\
@@ -233,8 +253,7 @@ val lemma_extendcut_prev
   (d:bin_tree_node{points_to_none pf d})
   (a:bin_tree_node{is_proper_desc d a /\ 
                     points_to_some pf a (desc_dir d a) /\
-                    is_proper_desc (pointed_node pf a (desc_dir d a)) d /\ 
-                    root_reachable pf a})
+                    is_proper_desc (pointed_node pf a (desc_dir d a)) d})
   (n:bin_tree_node):
   Lemma (requires (root_reachable pf n /\ n <> Root /\ n <> d /\ n <> pointed_node pf a (desc_dir d a)))
         (ensures (root_reachable (extendcut_ptrfn pf d a) n /\
@@ -262,12 +281,3 @@ val lemma_extendcut_prev2
                   root_reachable (extendcut_ptrfn pf d a) (pointed_node pf a (desc_dir d a)) /\
                   d = prev_in_path (extendcut_ptrfn pf d a) (pointed_node pf a (desc_dir d a)) Root)
 
-(* 
- * The setup is (Root -> a) and (Root -> d) and d is a proper descendant of a, 
- * then a points to some ancestor of d 
- *)
-val lemma_reachable_between (pf: ptrfn) (d: bin_tree_node) (a: bin_tree_node):
-  Lemma (requires (root_reachable pf d /\ is_proper_desc d a /\ root_reachable pf a))
-        (ensures (let c = desc_dir d a in
-                  points_to_some pf a c /\ 
-                  is_desc d (pointed_node pf a c))) 
